graph.md
@@ -4,9 +4,6 @@ graph TD;
   pure --> specs[specifications];
   lang --> specs;
   specs -->  pers[persistently];
-  specs --> later;
-  pers -->  ra[resource algebra];
-  later --> invariants;
   ra --> cst_ra[custom resource algebra];
   ra --> invariants;
   invariants --> conc[concurrency];
@@ -16,13 +13,17 @@ graph TD;
   spinlock --> ticketlock;
   spinlock --> adequacy;
 
-  specs --> linklist[linked list];
+  pers --> linklist[linked list];
+  pers -->  ra[resource algebra];
+
+  specs --> later;
+  later --> invariants;
   later --> fix[fixpoint];
   linklist --> fix[fixpoint];
 
   linklist --> arrays;
-  arrays --> merge[merge sort];
   conc --> merge;
+  arrays --> merge[merge sort];
 
   ofe;
 ```
